SimAsm/SimAsm_State.thy
@@ -1,15 +1,31 @@
 theory SimAsm_State
-  imports Main
+  imports Main "../Push_State"
 begin
 
 section \<open>State\<close>
 
 
-(* variable: either a register or a global. *)
+(* variable: either a register or a global, where registers equal local vars *)
+datatype 'r Reg = reg 'r | tmp 'r
 datatype ('g,'r) var = Reg 'r | Glb 'g
 
+text \<open> A state record is a partial mapping from vars to values, st
+         capture set, cap, denotes the set of "new" variables that the frame quantifies over
+         (these are the variables updated in the framed code)
+       state_rec describes the current "frame" on which an inst operates over, 
+         including mappings to variables that are existentially bound within the current 
+         "context" 
+       useful to model transient buffers which frame mis-speculated executions
+         of a branch which should not take effect on actual (core) mem but should reside
+         within its "local" frame; 
+       \<close>
+record ('v,'a) state_rec = st :: "'a \<Rightarrow> 'v option"
+                           cap :: "'a set"
+(*
 (* state record mapping some key (for example a variable name) to values *)
 record ('v,'a) state_rec = st :: "'a \<Rightarrow> 'v"
+*)
+
 
 (* because records can be arbitrarily extended, a record automatically gives rise to a
 *_scheme type which defines arbitrary possible extensions to that record.
@@ -39,9 +55,29 @@ type_synonym ('v,'g,'r,'a) rtrans = "('v,'g,'r,'a) trel \<Rightarrow> ('v,'g,'r,
 (* the possible extension of the state is used to store this auxiliary information *)
 type_synonym ('v,'g,'r,'a) auxfn = "('v,('g,'r) var,'a) state_rec_scheme \<Rightarrow> 'a"
 
+(* obtains the global state *)
+definition glb :: "('v,'g,'r,'a) state \<Rightarrow> ('g \<Rightarrow> 'v option)"
+  where "glb m \<equiv> \<lambda>v. st m (Glb v)"
+
+definition rg :: "('v,'g,'r,'a) state \<Rightarrow> ('r \<Rightarrow> 'v option)"
+  where "rg m \<equiv> \<lambda>v. st m (Reg v)"
+
+definition aux
+  where "aux m \<equiv> more m"
+
+text \<open>Domain of register variables\<close>
+
+(* Tmp registers are also local? *)
+abbreviation locals
+  where "locals \<equiv> Reg ` UNIV"
+
+text \<open>Domain of register variables\<close>
+abbreviation globals
+  where "globals \<equiv> Glb ` UNIV"
+
 section \<open>Write Operations\<close>
                                            
-definition st_upd :: "('v,'a,'b) state_rec_scheme \<Rightarrow> 'a \<Rightarrow> 'v \<Rightarrow> ('v,'a,'b) state_rec_scheme"
+definition st_upd :: "('v,'a,'b) state_rec_scheme \<Rightarrow> 'a \<Rightarrow> 'v option \<Rightarrow> ('v,'a,'b) state_rec_scheme"
   where "st_upd m a b = m \<lparr> st := ((st m) (a := b)) \<rparr>"
 
 definition aux_upd :: "('v,'r,'a) state_rec_scheme \<Rightarrow> (('v,'r,'a) state_rec_scheme \<Rightarrow> 'a) \<Rightarrow> ('v,'r,'a) state_rec_scheme"
@@ -61,28 +97,55 @@ translations
   "f(x:=\<^sub>sy)" \<rightleftharpoons> "CONST st_upd f x y"
   "f(aux: y)" \<rightleftharpoons> "CONST aux_upd f y"
 
+section \<open>Simp Lemmas\<close>
+
 lemma [simp]:
   "st (m(r :=\<^sub>s e)) q = (if r = q then e else st m q)"
   by (auto simp: st_upd_def)
+
+lemma [simp]:
+  "st (m(v :=\<^sub>s e)) = (st m)(v := e)"
+  by (auto simp: st_upd_def)
+
+lemma [simp]:
+  "more (m(aux: e)) = e m"
+  by (auto simp: aux_upd_def)
+
+lemma [simp]:
+  "rg (m(Glb x :=\<^sub>s e)) = rg m"
+  by (auto simp: rg_def st_upd_def)
+
+lemma [simp]:
+  "rg (m(Reg x :=\<^sub>s e)) = (rg m)(x := e)"
+  by (auto simp: st_upd_def rg_def)
 
 lemma aux_nop [simp]:
   "m(aux:more) = m"
   by (auto simp: aux_upd_def)
 
+lemma aux_st [simp]:
+  "st (m(aux: e)) = st m"
+  by (auto simp: aux_upd_def)
+
 lemma st_upd_twist: "a \<noteq> c \<Longrightarrow> (m(a :=\<^sub>s b))(c :=\<^sub>s d) = (m(c :=\<^sub>s d))(a :=\<^sub>s b)"
   unfolding st_upd_def by (auto intro!: equality fun_upd_twist)
 
-(* obtains the global state *)
-definition glb :: "('v,'g,'r,'a) state \<Rightarrow> ('v,'g,'a) gstate"
-  where "glb m \<equiv> \<lparr> st = (\<lambda>v. st m (Glb v)), \<dots> = more m \<rparr>"
-
-(* obtains the register state as a usual function. *)
-definition rg :: "('v,'g,'r,'a) state \<Rightarrow> 'r \<Rightarrow> 'v"
-  where "rg m \<equiv> \<lambda>v. st m (Reg v)"
 
 lemma [simp]:
   "glb (m(Reg r :=\<^sub>s e)) = glb m"
   by (auto simp: glb_def st_upd_def)
+
+lemma [simp]:
+  "glb (m(Reg r :=\<^sub>s e, aux: f)) = glb (m(aux: \<lambda>m. f(m(Reg r :=\<^sub>s e))))"
+  by (auto simp: aux_def glb_def)
+
+lemma [simp]:
+  "st m (Reg x) = rg m x"
+  by (auto simp: rg_def)
+
+lemma [simp]:
+  "aux (m(Reg x :=\<^sub>s e)) = aux m"
+  by (auto simp: aux_def st_upd_def)
 
 lemma [simp]:
   "P O {(m, m'). m' = m} = P"
@@ -96,18 +159,169 @@ lemma [simp]:
   "state_rec.more (m(aux: f)) = f m"
   by (auto simp: aux_upd_def)
 
-(* what is this? *)
 lemma aux_exec [intro!]:
   assumes "(m\<^sub>1,m\<^sub>2) \<in> P"
   shows "(m\<^sub>1,m\<^sub>2(aux: f)) \<in> P O {(m, m'). m' = m(aux: f)}"
   using assms by blast
 
-text \<open>Domain of register variables\<close>
-abbreviation locals
-  where "locals \<equiv> Reg ` UNIV"
 
-text \<open>Domain of register variables\<close>
-abbreviation globals
-  where "globals \<equiv> Glb ` UNIV"
+text \<open> stateTree as data structure in which each leaf is a state record;
+       the Base (initial leaf) has a mapping for all variables s \<mapsto> Some v
+          and it maintains all globally observable updates;
+       the top-most/right-most state record serves as a "frame" or "scope" 
+          to the current computation and gets discarded once the frame is exited;
+
+       stateTree is instantiated as a Push state;
+       the push operation creates a new sibling frame (to current frame) 
+         in which all mappings from m are set to None (all vars are undefined); 
+       when reading a variable within a frame and it is not yet defined in the current
+         "topmost" frame then a lookup routine goes through the recTree in reverse 
+         order of its build until it finds the innermost value available;
+       the record entry cap is the set of variables "captured/pushed/quantified"
+         in the current frame;
+       Globally visible updates (but only those) have to be stored in the Base, 
+         e.g. Cache; global stores in general are not observable since they
+         are not written to memory when speculating;
+       \<close>
+
+datatype  'n tree = Base 'n | Branch "'n tree" "'n tree"
+
+instantiation "tree" :: (state) state
+begin
+definition  
+      push_rec_def: "push m s = Branch m s"   (* pushes s on top of current tree t *) 
+
+instance proof
+  fix m m' s s':: "'a tree"
+  show "push m s = push m' s' \<Longrightarrow> (m = m' \<and> s = s')" 
+    by (simp add: push_rec_def)
+qed
+end
+
+type_synonym ('v,'g,'r,'a) stateTree = "(('v,('g,'r) var,'a) state_rec_scheme) tree"
+
+type_synonym ('v,'g,'r,'a) predTree = "('v,'g,'r,'a) stateTree set"
+
+type_synonym ('v,'r,'a) gstateTree = "(('v,'v,'a) state_rec_scheme) tree"
+type_synonym ('v,'a) gpredTree = "('v,'v,'a) gstateTree set"
+
+
+
+subsection \<open>Tree base, top and lookup and tree update\<close>
+
+fun base :: "('v,'g,'r,'a) stateTree \<Rightarrow> ('v,'g,'r,'a) state" where
+  "base (Base s) = s" |
+  "base (Branch m m') = (base m)"
+
+fun top :: "('v,'g,'r,'a) stateTree \<Rightarrow> ('v,'g,'r,'a) state" where
+  "top (Base s) = s" |
+  "top (Branch m m') = (case m' of (Base s) \<Rightarrow> s | _ \<Rightarrow> (top m'))"
+
+text \<open> lookup of var in a stateTree finds the closest (topmost) frame in which var is defined 
+         and returns its value in that frame \<close>
+fun lookup :: "('v,'g,'r,'a) stateTree \<Rightarrow> ('g,'r) var \<Rightarrow> 'v option" where
+  "lookup (Base s) var =  st s var" |
+  "lookup (Branch m m') var =
+                      (case (lookup m' var) of Some v \<Rightarrow> Some v |_ \<Rightarrow> lookup m var)"
+
+definition top_upd :: "('v,'g,'r,'a) stateTree \<Rightarrow> ('g,'r) var \<Rightarrow> 'v option \<Rightarrow> ('v,'g,'r,'a) stateTree" where
+  "top_upd t r val = Base (st_upd (top t) r val)"
+
+fun tree_upd :: "('v,'g,'r,'a) stateTree \<Rightarrow> ('v,'g,'r,'a) stateTree \<Rightarrow> ('v,'g,'r,'a) stateTree" where
+  "tree_upd (Base s) newTop = newTop" |
+  "tree_upd (Branch m m') newTop = (Branch m (tree_upd m' newTop))"
+
+
+subsection \<open> tree lemmas \<close>
+
+lemma [simp]: 
+  "tree_upd t (Base (top t)) = t" 
+proof (induction t)
+  case (Base x)
+  then show ?case by auto
+next
+  case (Branch t1 t2)
+  then show ?case apply auto
+    by (metis top.elims tree.simps(5) tree.simps(6))
+qed
+
+
+lemma stUpd_single :
+   "x \<noteq> r  \<Longrightarrow> st (st_upd m r v) x = st m x" by auto
+
+lemma topUpd_single:
+ "x \<noteq> r  \<Longrightarrow> lookup (top_upd (Base s) r (the val)) x = lookup (Base s) x"
+  using top_upd_def stUpd_single by (metis(full_types) lookup.simps(1) top.simps(1))
+   
+lemma treeUpd_change: 
+  "x \<noteq> r  \<Longrightarrow> lookup (tree_upd t (top_upd t r (the val))) x = lookup t x"
+proof (induct t)
+  case (Base s)
+  then show ?case using topUpd_single lookup.simps(1) by fastforce
+next
+  case (Branch t1 t2)
+  then show ?case using topUpd_single lookup.simps(2) top.elims top_upd_def tree.distinct(1) 
+             tree.inject(2) tree.simps(5) tree.simps(6) tree_upd.simps(2)
+    by (smt (verit, ccfv_threshold) )
+qed
+
+lemma top_treeUpd:
+    "top (tree_upd t (Base newTop)) = newTop" 
+proof (induction t)
+  case (Base x)
+  then show ?case by simp
+next
+  case (Branch t1 t2)
+  then show ?case 
+  proof (induction t2)
+    case (Base x)
+    then show ?case by simp
+  next
+    case (Branch t21 t22)
+    then show ?case by auto
+  qed
+qed
+
+lemma lookup_upd:
+  "val \<noteq> None \<Longrightarrow> lookup (tree_upd t (top_upd t r val)) r = val"
+proof (induction t)
+  case (Base x)
+  then show ?case using lookup.simps(1) tree_upd.simps(1) top_treeUpd topUpd_single
+    by (simp add: top_upd_def)
+next
+  case (Branch t1 t2)
+  then show ?case 
+  proof (induction t2)
+    case (Base x)
+    then show ?case using tree_upd.simps lookup.simps(2) top.simps tree.simps(5)
+      by (metis (no_types, lifting) option.case_eq_if option.collapse top_upd_def)
+  next
+    case (Branch t21 t22)
+    then show ?case using tree_upd.simps(2) lookup.simps(2) top.simps tree.simps(2,6)
+      by (metis (mono_tags, lifting) option.case_eq_if option.collapse top_upd_def)
+  qed
+qed
+
+
+
+(* new tree def: local state on top of tree *)
+definition rgTree :: "('v,'g,'r,'a) stateTree \<Rightarrow> ('r \<Rightarrow> 'v option)"
+  where "rgTree t \<equiv> \<lambda>v. st (top t) (Reg v)"
+
+
+(* obtains the global state of current tree *)
+definition glb\<^sub>t :: "('v,'g,'r,'a) stateTree \<Rightarrow> ('g \<Rightarrow> 'v option)"
+  where "glb\<^sub>t t \<equiv> \<lambda>v. (lookup t) (Glb v)"
+
+(* local state of current tree *)
+definition rg\<^sub>t :: "('v,'g,'r,'a) stateTree \<Rightarrow> ('r \<Rightarrow> 'v option)"
+  where "rg\<^sub>t t \<equiv> \<lambda>v. (lookup t) (Reg v)"
+
+
+(* ? what do we want here? *)
+
+definition aux\<^sub>t 
+  where "aux\<^sub>t t \<equiv> (lookup t) more"
+
 
 end
