SimAsm/SimAsm_WP.thy
@@ -123,66 +123,43 @@ definition w
 
 
 text \<open>Convert the language into the abstract language expected by the underlying logic\<close> 
-fun lift\<^sub>c :: "('v,'g,'r,'a) lang \<Rightarrow> (('v,'g,'r,'a) auxop, ('v,'g,'r,'a) state) com"
+fun lift\<^sub>c :: "('v,'g,'r,'a) lang \<Rightarrow> (('v,'g,'r,'a) auxop, ('v,'g,'r,'a) state) com" 
   where
     "lift\<^sub>c Skip = com.Nil" |
     "lift\<^sub>c (Op v a f) = Basic (\<lfloor>v,a,f\<rfloor>)" |
     "lift\<^sub>c (lang.Seq c\<^sub>1 c\<^sub>2) = (com.Seq (lift\<^sub>c c\<^sub>1) w (lift\<^sub>c c\<^sub>2))" |   (* lang.seq no wmm *)
-    "lift\<^sub>c (If b c\<^sub>1 c\<^sub>2) = (Choice (\<lambda> state. if (eval\<^sub>b b state) then (* fix me *)
-                     (com.Seq (Basic (\<lfloor>cmp b\<rfloor>)) w (lift\<^sub>c c\<^sub>1)) else 
-                     (com.Seq (Basic (\<lfloor>ncmp b\<rfloor>)) w (lift\<^sub>c c\<^sub>2))))" |
-    "lift\<^sub>c (While b I c) = (com.Seq ((com.Seq (Basic (\<lfloor>cmp b\<rfloor>))*\<^sub>w) (lift\<^sub>c c)) (Basic (\<lfloor>ncmp b\<rfloor>)))" | 
-    "lift\<^sub>c (DoWhile I c b) = (((lift\<^sub>c c ;\<^sub>w (Basic (\<lfloor>cmp b\<rfloor>)))*\<^sub>w) ;\<^sub>w lift\<^sub>c c) ;\<^sub>w (Basic (\<lfloor>ncmp b\<rfloor>))" 
+    "lift\<^sub>c (If b c\<^sub>1 c\<^sub>2) = (Choice (\<lambda> state. if (ev\<^sub>B state b)       
+                                 then (com.Seq (Basic (\<lfloor>cmp b\<rfloor>)) w (lift\<^sub>c c\<^sub>1)) 
+                                 else (com.Seq (Basic (\<lfloor>ncmp b\<rfloor>)) w (lift\<^sub>c c\<^sub>2))))" |
+    "lift\<^sub>c (While b I c) = (((Basic (\<lfloor>cmp b\<rfloor>)) ;\<^sub>w (lift\<^sub>c c))*\<^sub>w) ;\<^sub>w (Basic (\<lfloor>ncmp b\<rfloor>))" | 
+    "lift\<^sub>c (DoWhile I c b) = ((((lift\<^sub>c c) ;\<^sub>w (Basic (\<lfloor>cmp b\<rfloor>)))*\<^sub>w) ;\<^sub>w (lift\<^sub>c c)) ;\<^sub>w (Basic (\<lfloor>ncmp b\<rfloor>))" 
 
-text \<open>Correctness of the guarantee check\<close>
-lemma com_guar:
-  "wellformed R G \<Longrightarrow> guar\<^sub>c c G \<Longrightarrow> \<forall>\<beta>\<in>basics (lift\<^sub>c c). guar\<^sub>\<alpha> \<beta> (step G)"
-proof (induct c)
-  case Skip
-  then show ?case sorry
-next
-  case (Op pred op aux)
-  then show ?case 
-    apply (cases op) 
-       apply (auto simp: liftg_def guar_def wp\<^sub>r_def) 
-    sorry
-next
-  case (Seq c1 c2)
-  then show ?case sorry
-next
-  case (If x1 c1 c2)
-  then show ?case sorry
-next
-  case (While x1 x2 c)
-  then show ?case sorry
-next
-  case (DoWhile x1 c x3)
-  then show ?case sorry
-qed 
-(* (auto simp: guar_def reflexive_def liftl_def step_def) *)
- 
 
 (* these two dummy parameters used in the interpretation of rules
     and help to instantiate the types of auxop and state for ARMv8 *)
 
 abbreviation "someAuxOp ::('v,'g,'r,'a) auxop  \<equiv> undefined"
-abbreviation "someState :: ('v,'g,'r,'a) state \<equiv> undefined" 
+abbreviation "someState :: ('v,'g,'r,'a) state \<equiv> undefined" (* add a push instance *)
+abbreviation "someAuxOp_someState :: (('v,'g,'r,'a) auxop \<times> ('v,'g,'r,'a) state)  \<equiv> undefined"
 
 print_locale rules
 
-interpretation rules "someAuxOp" 
+(*Type unification failed: No type arity state_rec_ext :: state , when adding parameter someState *)
+
+interpretation rules "someAuxOp" "someState"
   by (unfold_locales)
 
 
-(*
-interpretation rules fwd\<^sub>s re\<^sub>a 
-  apply (unfold_locales)
-  apply (auto)
-  apply (case_tac ad)
-  apply auto
-  (* apply (auto simp: Let_def) *)
-  done
-*)
+text \<open>Correctness of the guarantee check\<close>
+lemma com_guar:
+  "wellformed R G \<Longrightarrow> guar\<^sub>c c G \<Longrightarrow>  \<forall>\<beta> \<in> obs (lift\<^sub>c c). guar\<^sub>\<alpha> \<beta> (step G)"
+proof (induct c)
+  case (Op pred op aux)
+  then show ?case  
+    apply (cases op) using Op  
+       by (auto simp: liftg_def guar_def wp\<^sub>r_def) 
+qed (auto simp: guar_def reflexive_def liftl_def step_def) 
+
 
 text \<open>Extract the instruction from an abstract operation\<close>
 abbreviation inst :: "('v,'g,'r,'a) opbasic \<Rightarrow> ('v,'g,'r) op"
