SimAsm/SimAsm.thy
@@ -1,5 +1,5 @@
 theory SimAsm
-  imports  "../Security"  SimAsm_Exp
+  imports  "../Soundness"  SimAsm_Exp
 begin
 
 text \<open>Instruction Reordering\<close>
